\chapter{Distance measures for quantum information}

\section{Distance measures for classical information}

\ex pass.

\ex pass.

\ex pass.

\ex Let $S_+ =\{x:p_x>q_x\}$ and $S_- =\{x:p_x<q_x\}$.
Then,
$$\sum_{x\in S_+}(p_x-q_x)-\sum_{x\in S_-}(q_x-p_x)=\sum_x(p_x-q_x)=\sum_xp_x-\sum_xq_x=0,$$
i.e., $\sum_{x\in S_+}(p_x-q_x)=\sum_{x\in S_-}(q_x-p_x)$.

One one hand, we have
$$D(p_x,q_x) = \frac{1}{2}\sum_x|p_x-q_x| = \frac{1}{2}\left(\sum_{x\in S_+}(p_x-q_x)+\sum_{x\in S_-}(q_x-p_x)\right) = \sum_{x\in S_+}(p_x-q_x).$$

On the other hand, it is obvious that
$$\max_S\left|\sum_{x\in S}(p_x-q_x)\right| = \max\left(\sum_{x\in S_+}(p_x-q_x), \sum_{x\in S_-}(q_x-p_x)\right) = \sum_{x\in S_+}(p_x-q_x).$$

Hence the desired equality is obtained.

\ex Similar to the previous exercise, we have
$$\max_S\left|\sum_{x\in S}(p_x-q_x)\right| = \sum_{x\in S_+}(p_x-q_x) = D(p_x, q_x).$$
